more

Mazza2.thy
@@ -1,9 +1,24 @@
-theory Mazza
+theory Mazza2
   imports
     "thys/MRBNF_Recursor"
-    Countably_Infinite_Set
-    Countably_Infinite_Multiset
+    "HOL-Library.Stream"
+    "HOL-Library.Countable_Set_Type"
+    "HOL-Cardinals.Cardinals"
 begin
+
+class infinite_regular =
+  assumes large: "|Field (card_suc natLeq)| \<le>o |UNIV::'a set|" and regular: "regularCard |UNIV::'a set|"
+
+lemma infinite_natLeq: "natLeq \<le>o |A| \<Longrightarrow> infinite A"
+  using infinite_iff_natLeq_ordLeq by blast
+
+lemma infinite: "infinite (UNIV :: 'a ::infinite_regular set)"
+  using ordLeq_transitive[OF ordLess_imp_ordLeq[OF card_suc_greater_set[OF natLeq_card_order ordLeq_refl[OF natLeq_Card_order]]]
+      ordIso_ordLeq_trans[OF ordIso_symmetric[OF card_of_Field_ordIso[OF Card_order_card_suc[OF natLeq_card_order]]] large]]
+  by (rule infinite_natLeq)
+
+lemma infinite_ex_inj: "\<exists>f :: nat \<Rightarrow> 'a :: infinite_regular. inj f"
+  by (rule infinite_countable_subset[OF infinite, simplified])
 
 (*untyped lambda calculus*)
 (* binder_datatype 'a lam =
@@ -35,6 +50,51 @@ val spec_lam = {
 }
 \<close>
 
+coinductive sdistinct where
+  "x \<notin> sset s \<Longrightarrow> sdistinct s \<Longrightarrow> sdistinct (x ## s)"
+
+lemma sdistinct_stl: "sdistinct s \<Longrightarrow> sdistinct (stl s)"
+  by (erule sdistinct.cases) simp
+
+lemma sdistinct_fromN[simp]: "sdistinct (fromN n)"
+  by (coinduction arbitrary: n) (subst siterate.code,  auto)
+
+lemma sdistinct_smap: "inj_on f (sset s) \<Longrightarrow> sdistinct s \<Longrightarrow> sdistinct (smap f s)"
+  by (coinduction arbitrary: s)
+    (auto simp: smap_ctr stream.set_map inj_on_def stream.set_sel sdistinct_stl elim: sdistinct.cases)
+
+typedef 'a dstream = "{xs :: 'a :: infinite_regular stream. sdistinct xs}"
+  by (auto intro!: exI[of _ "smap (SOME f :: nat \<Rightarrow> 'a. inj f) nats"] sdistinct_smap
+    someI_ex[OF infinite_ex_inj])
+
+setup_lifting type_definition_dstream
+
+lift_definition map_dstream :: "('a \<Rightarrow> 'a) \<Rightarrow> 'a dstream \<Rightarrow> 'a :: infinite_regular dstream" is
+  "\<lambda>f xs. if bij f then smap f xs else xs"
+  by (auto simp: bij_def intro!: sdistinct_smap elim: inj_on_subset)
+
+lift_definition set_dstream :: "'a :: infinite_regular dstream \<Rightarrow> 'a set" is "sset" .
+
+mrbnf "'a ::infinite_regular dstream"
+  map: map_dstream
+  sets: bound: set_dstream
+  bd: natLeq
+  var_class: infinite_regular
+  subgoal apply (rule ext, transfer)
+    using [[show_consts]]
+    apply simp
+(*
+  subgoal by (rule ext, transfer) simp
+  subgoal by transfer simp
+  subgoal by (rule ext, transfer) simp
+  subgoal by (rule infinite_regular_card_order_natLeq)
+  subgoal by transfer (simp flip: finite_iff_ordLess_natLeq)
+  subgoal by blast
+  subgoal by (clarsimp, transfer) auto
+  done
+*)
+*)
+
 declare [[mrbnf_internals]]
 local_setup \<open> MRBNF_Sugar.create_binder_datatype spec_lam \<close>
 print_mrbnfs
@@ -45,8 +105,8 @@ abbreviation "fv \<equiv> FFVars_lam"
 (* binder_datatype 'a ilam =
   Bot
 | Var 'a
-| App "'a ilam" "'a ilam cinfmset"
-| Abs "X::'a cinfset" "t::'a ilam" binds X in t
+| App "'a ilam" "'a ilam stream"
+| Abs "X::'a dstream" "t::'a ilam" binds X in t
 *)
 
 ML \<open>
@@ -100,6 +160,7 @@ lemma iso_partition_into_countable: "|UNIV :: 'a :: var_ilam_pre set| *c natLeq 
   by (rule cprod_infinite1'[OF _ Cinfinite_Cnotzero[OF natLeq_Cinfinite]])
     (simp_all add: var_ilam_pre_class.cinfinite var_sum_class.large)
 
+
 definition iso_partition where
   "iso_partition = (SOME f:: 'a :: var_ilam_pre \<Rightarrow> nat \<Rightarrow> 'a. bij_betw (case_prod f) UNIV UNIV)"
 
@@ -116,7 +177,7 @@ lemma partition_var_partition: "partition_on UNIV var_partition"
   using bij_iso_partition unfolding bij_def surj_def inj_on_def
   by (auto 5 5)
 
-lemma inj_iso_partition: "inj (iso_partition x)"
+lemma inj_iso_partition: "inj (iso_partition X)"
   using bij_iso_partition unfolding bij_def inj_on_def
   by auto
 
@@ -127,119 +188,34 @@ lemma var_partition_cinf: "X \<in> var_partition \<Longrightarrow> countable X \
 lemma ex1_var_partition: "\<exists>!X. X \<in> var_partition \<and> x \<in> X"
   using partition_var_partition unfolding partition_on_def disjoint_def by auto
 
-lemma Union_var_partition: "(\<Union>X \<in> var_partition. X) = UNIV"
-  using ex1_var_partition by fast
+lift_definition super :: "'a ::var_ilam_pre \<Rightarrow> 'a cinfset" ("\<lbrace>_\<rbrace>" [999] 1000) is
+  "\<lambda>x. THE X. X \<in> var_partition \<and> x \<in> X"
+  by (rule the1I2[OF ex1_var_partition]) (auto simp: var_partition_cinf)
 
-lemma natLeq_less_UNIV: "natLeq <o |UNIV :: 'a :: var_ilam_pre set|"
-  apply (rule ordLess_ordLeq_trans[OF _ ilam.var_large])
-  apply (rule ordLess_ordIso_trans[OF card_suc_greater[OF natLeq_card_order]])
-  apply (tactic \<open>BNF_Tactics.unfold_thms_tac @{context} [Thm.axiom @{theory} "Mazza.ilam_pre.bd_ilam_pre_def"]\<close>)
-  apply (rule ordIso_transitive[OF _ dir_image_ordIso])
-    apply (rule ordIso_symmetric)
-    apply (rule ordIso_transitive)
-     apply (rule cprod_infinite1')
-       apply (simp add: Cinfinite_csum Field_natLeq natLeq_card_order natLeq_cinfinite)
-      apply (simp add: lam_pre.bd_Cnotzero)
-     apply (simp add: Field_natLeq natLeq_card_order ordLeq_csum1)
-    apply (rule ordIso_transitive)
-     apply (rule csum_absorb2)
-      apply (simp add: Card_order_cprod Cinfinite_csum1 cinfinite_cprod natLeq_Cinfinite)
-     apply (simp add: Card_order_cprod Cinfinite_csum1 cinfinite_cprod natLeq_Cinfinite natLeq_ordLeq_cinfinite)
-    apply (rule ordIso_transitive)
-     apply (rule cprod_infinite1')
-       apply (simp add: Card_order_csum cinfinite_cprod cinfinite_csum natLeq_Cinfinite)
-      apply (simp add: lam_pre.bd_Cnotzero)
-     apply (simp add: Card_order_csum cinfinite_cprod cinfinite_csum natLeq_Cinfinite natLeq_ordLeq_cinfinite)
-    apply (rule ordIso_transitive)
-     apply (rule csum_absorb2)
-      apply (simp add: Card_order_cprod cinfinite_cprod cinfinite_csum natLeq_Cinfinite)
-     apply (simp add: cprod_cong1 csum_com ordIso_imp_ordLeq)
-    apply (rule ordIso_transitive)
-     apply (rule cprod_infinite1')
-       apply (simp add: Card_order_csum cinfinite_csum natLeq_Cinfinite)
-      apply (simp add: lam_pre.bd_Cnotzero)
-     apply (simp add: natLeq_Cinfinite ordLeq_csum2)
-    apply (simp add: csum_absorb1 infinite_regular_card_order.Card_order infinite_regular_card_order.cinfinite infinite_regular_card_order_card_suc natLeq_Cinfinite natLeq_card_order natLeq_ordLeq_cinfinite)
-  using Card_order_cprod card_order_on_well_order_on apply blast
-  apply (simp add: inj_on_def Abs_ilam_pre_bdT_inject)
-  done
+lemma in_super: "x \<in>\<in> \<lbrace>x\<rbrace>"
+  by transfer (rule the1I2[OF ex1_var_partition, THEN conjunct2])
 
-lemma infinite_var_partition: "infinite (var_partition :: 'a :: var_ilam_pre set set)"
-  apply (rule notI)
-  apply (subgoal_tac "countable (UNIV :: 'a :: var_ilam_pre set)")
-  using natLeq_less_UNIV not_ordLeq_ordLess countable_card_le_natLeq apply blast
-  apply (auto simp: Union_var_partition[symmetric] countable_finite
-    dest: var_partition_cinf intro!: countable_UN[of _ "\<lambda>X. X", simplified])
-  done
+lemma super_in: "set_cinfset \<lbrace>x\<rbrace> \<in> var_partition"
+  by transfer (rule the1I2[OF ex1_var_partition, THEN conjunct1])
 
-lemma var_partition_ordIso: "|var_partition :: 'a :: var_ilam_pre set set| =o |UNIV :: 'a set|"
-  unfolding ordIso_iff_ordLeq
-  apply (rule conjI)
-   apply (unfold var_partition_def) []
-   apply (rule card_of_image)
-  apply (unfold Union_var_partition[symmetric])
-  apply (rule card_of_UNION_ordLeq_infinite)
-    apply (auto simp: infinite_var_partition)
-   apply (drule var_partition_cinf)
-  apply (auto simp: countable_card_le_natLeq elim!: ordLeq_transitive)
-  using infinite_iff_natLeq_ordLeq infinite_var_partition by blast
-
-lift_definition cinf_partition :: "'a :: var_ilam_pre cinfset set" is "var_partition"
-  by (auto dest: var_partition_cinf)
-
-lemma cinf_partition_disjoint:
-  "X \<in> cinf_partition \<Longrightarrow> Y \<in> cinf_partition \<Longrightarrow> X \<noteq> Y \<Longrightarrow> set_cinfset X \<inter> set_cinfset Y = {}"
-  by transfer (meson disjoint_def partition_on_def partition_var_partition)
-
-definition super :: "'a ::var_ilam_pre \<Rightarrow> 'a cinfset" ("\<lbrace>_\<rbrace>" [999] 1000) where
-  "super = (SOME f. bij_betw f UNIV cinf_partition)"
-
-lemma bij_betw_super: "bij_betw super (UNIV :: 'a :: var_ilam_pre set) cinf_partition"
-  unfolding super_def
-  apply (rule someI_ex[of "\<lambda>f. bij_betw f UNIV cinf_partition"])
-  apply (rule card_of_ordIso[where 'a='a, THEN iffD2, OF ordIso_symmetric[OF var_partition_ordIso], THEN exE])
-  unfolding cinf_partition_def
-  subgoal for f
-    apply (rule exI[of _ "Abs_cinfset o f"])
-    apply (rule bij_betw_comp_iff2[THEN iffD1, rotated 2])
-    apply assumption
-     apply (rule inj_on_imp_bij_betw)
-     apply (auto simp: inj_on_def Abs_cinfset_inject dest!: var_partition_cinf elim: bij_betw_apply)
-    done
-  done
-
-lemma super_inject: "\<lbrace>x\<rbrace> = \<lbrace>y\<rbrace> \<Longrightarrow> x = y"
-  by (meson bij_betw_imp_inj_on bij_betw_super injD)
-
-lemma disjoint_super: "x \<noteq> y \<Longrightarrow> set_cinfset \<lbrace>x\<rbrace> \<inter> set_cinfset \<lbrace>y\<rbrace> = {}"
-  by (metis UNIV_I bij_betw_iff_bijections bij_betw_super cinf_partition_disjoint)
-
-lemma bij_betw_swap: "bij_betw f A B \<Longrightarrow> a \<in> A \<Longrightarrow> b \<in> A \<Longrightarrow>  bij_betw (f(a := f b, b := f a)) A B"
-  apply (auto simp: bij_betw_def image_iff)
-  apply (auto simp: inj_on_def)
-  done
-
+lemma disjoint_super: "\<lbrace>x\<rbrace> \<noteq> \<lbrace>y\<rbrace> \<Longrightarrow> set_cinfset \<lbrace>x\<rbrace> \<inter> set_cinfset \<lbrace>y\<rbrace> = {}"
+  by (metis Int_emptyI ex1_var_partition set_cinfset_inject super_in)
 
 typedef 'a :: var_ilam_pre super =
-   "{f :: 'a \<Rightarrow> 'a cinfset. bij_betw f UNIV cinf_partition \<and> (\<forall>x y. x \<noteq> y \<longrightarrow> set_cinfset (f x) \<inter> set_cinfset (f y) = {})}"
-  by (auto intro!: exI[of _ super] simp: bij_betw_super dest: disjoint_super)
+   "{f :: 'a \<Rightarrow> 'a cinfset. \<forall>x y. f x \<noteq> f y \<longrightarrow> set_cinfset (f x) \<inter> set_cinfset (f y) = {}}"
+  by (auto intro!: exI[of _ super] simp: in_super dest: disjoint_super)
 setup_lifting type_definition_super
 lift_definition apply_super :: "'a :: var_ilam_pre super \<Rightarrow> 'a \<Rightarrow> 'a cinfset" is "id :: _ \<Rightarrow> ('a \<Rightarrow> 'a cinfset)" .
 lift_definition comp_super :: "'a :: var_ilam_pre super \<Rightarrow> ('a \<Rightarrow> 'a) \<Rightarrow> 'a :: var_ilam_pre super" is
   "\<lambda>g f. if bij f then g o f else g"
-  by (auto simp: bij_betw_comp_iff2[symmetric])
+  by force
 lift_definition swap_super :: "'a :: var_ilam_pre super \<Rightarrow> 'a \<Rightarrow> 'a \<Rightarrow> 'a :: var_ilam_pre super" is
   "\<lambda>g z z'. g (z := g z', z' := g z)"
-  by (auto simp: bij_betw_swap split: if_splits)
+  by (auto split: if_splits)
 
-lemma swap_super_self[simp]: "swap_super g x x = g"
-  by transfer auto
-
-lemma apply_super_eqI:
+lemma apply_super_disjoint:
   "x \<in>\<in> apply_super g z \<Longrightarrow> x \<in>\<in> apply_super g z' \<Longrightarrow> apply_super g z = apply_super g z'"
-  apply transfer
-  apply auto
-  by (metis disjoint_iff)
+  by transfer auto
 
 lemma apply_super_swap_super[simp]: "apply_super (swap_super g z z') x =
   (if x = z then apply_super g z' else if x = z' then apply_super g z else apply_super g x)"
@@ -251,10 +227,6 @@ definition bij_cinfset where
   "bij_cinfset A B x = (if x \<in>\<in> A then get_cinfset B (idx_cinfset A x)
      else if x \<in>\<in> B then get_cinfset A (idx_cinfset B x)
      else x)"
-
-lemma bij_cinfset_self[simp]: "bij_cinfset X X = id"
-  unfolding bij_cinfset_def
-  by transfer auto
 
 lemma bij_betw_cinfset: "bij_betw (bij_cinfset A B) (set_cinfset A) (set_cinfset B)"
   unfolding bij_cinfset_def
@@ -289,7 +261,39 @@ subclass (in var_ilam_pre) var_lam_pre
   by standard
 
 lemma set_cinfset_bound: "|set_cinfset A :: 'a set| <o |UNIV :: 'a :: var_ilam_pre set|"
-  by (rule ordIso_ordLess_trans[OF card_of_set_cinfset natLeq_less_UNIV])
+  apply (rule ordIso_ordLess_trans[OF card_of_set_cinfset])
+  apply (rule ordLess_ordLeq_trans[OF _ ilam.var_large])
+  apply (rule ordLess_ordIso_trans[OF card_suc_greater[OF natLeq_card_order]])
+  apply (tactic \<open>BNF_Tactics.unfold_thms_tac @{context} [Thm.axiom @{theory} "Mazza.ilam_pre.bd_ilam_pre_def"]\<close>)
+  apply (rule ordIso_transitive[OF _ dir_image_ordIso])
+    apply (rule ordIso_symmetric)
+    apply (rule ordIso_transitive)
+     apply (rule cprod_infinite1')
+       apply (simp add: Cinfinite_csum Field_natLeq natLeq_card_order natLeq_cinfinite)
+      apply (simp add: lam_pre.bd_Cnotzero)
+     apply (simp add: Field_natLeq natLeq_card_order ordLeq_csum1)
+    apply (rule ordIso_transitive)
+     apply (rule csum_absorb2)
+      apply (simp add: Card_order_cprod Cinfinite_csum1 cinfinite_cprod natLeq_Cinfinite)
+     apply (simp add: Card_order_cprod Cinfinite_csum1 cinfinite_cprod natLeq_Cinfinite natLeq_ordLeq_cinfinite)
+    apply (rule ordIso_transitive)
+     apply (rule cprod_infinite1')
+       apply (simp add: Card_order_csum cinfinite_cprod cinfinite_csum natLeq_Cinfinite)
+      apply (simp add: lam_pre.bd_Cnotzero)
+     apply (simp add: Card_order_csum cinfinite_cprod cinfinite_csum natLeq_Cinfinite natLeq_ordLeq_cinfinite)
+    apply (rule ordIso_transitive)
+     apply (rule csum_absorb2)
+      apply (simp add: Card_order_cprod cinfinite_cprod cinfinite_csum natLeq_Cinfinite)
+     apply (simp add: cprod_cong1 csum_com ordIso_imp_ordLeq)
+    apply (rule ordIso_transitive)
+     apply (rule cprod_infinite1')
+       apply (simp add: Card_order_csum cinfinite_csum natLeq_Cinfinite)
+      apply (simp add: lam_pre.bd_Cnotzero)
+     apply (simp add: natLeq_Cinfinite ordLeq_csum2)
+    apply (simp add: csum_absorb1 infinite_regular_card_order.Card_order infinite_regular_card_order.cinfinite infinite_regular_card_order_card_suc natLeq_Cinfinite natLeq_card_order natLeq_ordLeq_cinfinite)
+  using Card_order_cprod card_order_on_well_order_on apply blast
+  apply (simp add: inj_on_def Abs_ilam_pre_bdT_inject)
+  done
 
 lemma supp_bij_cinfset[simp]:
   "|supp (bij_cinfset A B :: 'a \<Rightarrow> 'a)| <o |UNIV :: 'a :: var_ilam_pre set|"
@@ -298,26 +302,19 @@ lemma supp_bij_cinfset[simp]:
    apply (auto simp: set_cinfset_bound ilam.Un_bound)
   done
 
-lemma bij_betw_apply_super: "bij_betw (apply_super g) UNIV cinf_partition"
-  by transfer auto
-
-lemma apply_super_disjoint: "z \<noteq> z' \<Longrightarrow> set_cinfset (apply_super g z) \<inter> set_cinfset (apply_super g z') = {}"
-  by transfer auto
-
 abbreviation "eq_on_super g g' X \<equiv> \<forall>x \<in> X. apply_super g x = apply_super g' x"
 abbreviation "bij_super g z z' \<equiv> bij_cinfset (apply_super g z) (apply_super g z')"
 
 typedef 'a P_lam_ilam = "UNIV :: unit set" by auto
 typedef 'a :: var_ilam_pre U_lam_ilam = "{T :: 'a super \<Rightarrow> nat list \<Rightarrow> 'a ilam.
   (\<exists>X. finite X \<and> (\<forall>g g'. eq_on_super g g' X \<longrightarrow> T g = T g')
-     \<and> (\<forall>z z' g a. z' \<notin> X \<longrightarrow>
+     \<and> (\<forall>z z' g a. z \<in> X \<and> z' \<notin> X \<longrightarrow>
        ivvsubst (bij_super g z z') (T g a) = T (swap_super g z z') a))}"
   apply (rule exI[of _ "\<lambda>g a. iVar (get_cinfset (apply_super g undefined) (list_encode a))"] exI[of _ "{undefined}"] CollectI allI)+
   apply (auto 0 4 simp: infinite bij_cinfset_def get_cinfset_inverse idx_cinfset_inverse get_cinfset_in
-    dest: apply_super_eqI[OF get_cinfset_in] apply_super_eqI[OF _ get_cinfset_in])
-  apply (metis (mono_tags, lifting) Int_emptyD Rep_super apply_super.rep_eq get_cinfset_in mem_Collect_eq)
-  apply (metis (mono_tags, lifting) Int_emptyD Rep_super apply_super.rep_eq get_cinfset_in mem_Collect_eq)
+    dest: apply_super_disjoint[OF get_cinfset_in] apply_super_disjoint[OF _ get_cinfset_in])
   done
+
 
 setup_lifting type_definition_U_lam_ilam
 (*
@@ -373,24 +370,6 @@ lemma iAbs_inject: "(iAbs x e = iAbs x' e') = (\<exists>f :: 'a \<Rightarrow> 'a
   apply (auto simp: ilam_vvsubst_rrename)
   done
 
-lemma iVar_inject[simp]: "(iVar x = iVar x') = (x = x')"
-  unfolding ilam.set
-  unfolding iVar_def ilam.TT_injects0 map_ilam_pre_def comp_def Abs_ilam_pre_inverse[OF UNIV_I]
-    map_sum_def sum.case map_prod_def prod.case id_def Abs_ilam_pre_inject[OF UNIV_I UNIV_I] sum.inject prod.inject
-    set3_ilam_pre_def sum_set_simps Union_empty Un_empty_left prod_set_simps cSup_singleton set2_ilam_pre_def
-    Un_empty_right UN_single
-  apply (auto simp: ilam_vvsubst_rrename id_def[symmetric] cinfmset.map_id supp_id_bound intro!: exI[of _ id])
-  done
-
-lemma iApp_inject[simp]: "(iApp t U = iApp t' U') = (t = t' \<and> U = U')"
-  unfolding ilam.set
-  unfolding iApp_def ilam.TT_injects0 map_ilam_pre_def comp_def Abs_ilam_pre_inverse[OF UNIV_I]
-    map_sum_def sum.case map_prod_def prod.case id_def Abs_ilam_pre_inject[OF UNIV_I UNIV_I] sum.inject prod.inject
-    set3_ilam_pre_def sum_set_simps Union_empty Un_empty_left prod_set_simps cSup_singleton set2_ilam_pre_def
-    Un_empty_right UN_single
-  apply (auto simp: ilam_vvsubst_rrename id_def[symmetric] cinfmset.map_id supp_id_bound intro!: exI[of _ id])
-  done
-
 lemma image_cinfset_bij_cinfset:
   includes cinfset.lifting
   shows "image_cinfset (bij_cinfset A B) A = B"
@@ -399,28 +378,14 @@ lemma image_cinfset_bij_cinfset:
   apply (auto simp add: from_nat_into infinite_imp_nonempty image_iff inj_on_def)
   by (metis from_nat_into_surj to_nat_on_surj)
 
-lemma image_cinfset_bij_cinfset':
-  includes cinfset.lifting
-  assumes "set_cinfset A \<inter> set_cinfset B = {}"
-  shows "image_cinfset (bij_cinfset A B) B = A"
-  unfolding bij_cinfset_def using assms
-  apply transfer
-  apply (auto simp add: from_nat_into infinite_imp_nonempty image_iff inj_on_def)
-  by (metis Int_Collect Int_iff emptyE from_nat_into_surj to_nat_on_surj)
-
-lemma exist_fresh_super: "|A::'a set| <o |UNIV :: 'a :: var_ilam_pre set| \<Longrightarrow>
-  |B :: 'a set| <o |UNIV :: 'a :: var_ilam_pre set| \<Longrightarrow>
-  \<exists>a. a \<notin> A \<and> set_cinfset (apply_super g a) \<inter> B = {} \<and> set_cinfset (apply_super g' a) \<inter> B = {}"
-  sorry
-
-lemma iAbs_super_eqI: "finite X \<Longrightarrow>
+lemma iAbs_super_eqI: "|X :: 'a set| <o |UNIV :: 'a :: var_ilam_pre set| \<Longrightarrow>
   \<forall>g g'. (\<forall>x\<in>X. apply_super g x = apply_super g' x) \<longrightarrow> (\<forall>a. T g a = T g' a) \<Longrightarrow>
-  (\<forall>z z' g a. z' \<notin> X \<longrightarrow> ivvsubst (bij_cinfset (apply_super g z) (apply_super g z')) (T g a) = T (swap_super g z z') a) \<Longrightarrow>
+  (\<forall>z z' g a. z \<in> X \<and> z' \<notin> X \<longrightarrow>
+       ivvsubst (bij_cinfset (apply_super g z) (apply_super g z')) (T g a) = T (swap_super g z z') a) \<Longrightarrow>
   \<forall>y. y \<noteq> z \<longrightarrow> apply_super g y = apply_super g' y \<Longrightarrow>
   iAbs (apply_super g z) (T g a) = iAbs (apply_super g' z) (T g' a)"
-  apply (rule exist_fresh_super[THEN exE, of "insert z X" "ifv (T g a) \<union> ifv (T g' a)" g g'])
-    apply (meson finite_insert finite_ordLess_infinite2 infinite infinite_card_of_insert ordIso_ordLess_trans set_cinfset_bound var_lam_pre_class.Un_bound)
-  apply (meson ilam.set_bd_UNIV var_lam_pre_class.Un_bound)
+  apply (rule exists_fresh[THEN exE, of "insert z X \<union> set_cinfset (apply_super g z)"])
+  apply (meson finite_insert finite_ordLess_infinite2 infinite infinite_card_of_insert ordIso_ordLess_trans set_cinfset_bound var_lam_pre_class.Un_bound)
   subgoal for zz
     apply (rule box_equals[of
       "iAbs (apply_super (swap_super g z zz) z) (T (swap_super g z zz) a)"
@@ -437,31 +402,17 @@ lemma iAbs_super_eqI: "finite X \<Longrightarrow>
      apply (cases "apply_super g z = apply_super g zz")
     apply (smt (verit, ccfv_SIG) apply_super_swap_super)
     subgoal premises prems
-      using prems(5,3)
+      using prems(6)
       unfolding iAbs_inject
       apply (intro exI[of _ "bij_cinfset (apply_super g z) (apply_super g zz)"])
       apply (intro conjI)
           apply (rule bij_cinfset)
           apply transfer
-          apply fastforce
+          apply force
          apply (simp_all add: image_cinfset_bij_cinfset ilam_vvsubst_rrename[symmetric])
-      apply (auto simp: id_on_def bij_cinfset_def)
-      done
-     apply (rule sym)
-     apply (cases "apply_super g' z = apply_super g' zz")
-    apply (smt (verit, ccfv_SIG) apply_super_swap_super)
-    subgoal premises prems
-      using prems(5,3)
-      unfolding iAbs_inject
-      apply (intro exI[of _ "bij_cinfset (apply_super g' z) (apply_super g' zz)"])
-      apply (intro conjI)
-          apply (rule bij_cinfset)
-          apply transfer
-          apply fastforce
-         apply (simp_all add: image_cinfset_bij_cinfset ilam_vvsubst_rrename[symmetric])
-       apply (auto simp: id_on_def bij_cinfset_def)
-      done
-    done
+       prefer 2
+      sorry
+    sorry
   done
 
 lift_definition CCTOR_lam_ilam :: "('a::var_ilam_pre, 'a, 'a lam \<times> 'a PU_lam_ilam, 'a lam \<times> 'a PU_lam_ilam) lam_pre \<Rightarrow> 'a PU_lam_ilam" is
@@ -472,98 +423,112 @@ lift_definition CCTOR_lam_ilam :: "('a::var_ilam_pre, 'a, 'a lam \<times> 'a PU_
    | Inr (Inr (x, M)) \<Rightarrow> \<lambda>g a. iAbs (apply_super g x) (snd M u g a))"
   apply (tactic \<open>BNF_Tactics.unfold_thms_tac @{context} [Thm.axiom @{theory} "Mazza.lam_pre.rel_lam_pre_def"] \<close>)
   apply (tactic \<open>BNF_Tactics.unfold_thms_tac @{context} [Thm.axiom @{theory} "Mazza.lam_presum.sum2.sum.Sum_Type.rel_lam_presum_def"] \<close>)
-  apply (auto 0 0 simp only: fun_eq_iff vimage2p_def rel_sum.simps rel_fun_def rel_prod.simps split: sum.splits)
+  apply (auto 0 0 simp only: fun_eq_iff vimage2p_def rel_sum.simps rel_fun_def split: sum.splits)
   subgoal for lp1 lp2 x
     apply (rule exI[of _ "{x}"])
-    apply (auto simp add: bij_cinfset_def get_cinfset_in get_cinfset_inverse)
-    apply (metis Int_emptyD apply_super_disjoint idx_cinfset_inverse)
-    apply (meson Int_emptyD apply_super_disjoint get_cinfset_in)
-    apply (meson Int_emptyD apply_super_disjoint get_cinfset_in)
-    done
-  subgoal for lp1 lp2 M N TM2 TN2 TM1 TN1 u
-    apply (drule spec[of _ u])+
-    apply (drule mp, rule refl)+
+    apply auto
+    apply (metis (no_types, opaque_lifting) ilam.card_of_FFVars_bounds ilam.set(1) singletonI)
+  subgoal for lp1 lp2 M TM2 N TN2 TM1 TN1 u TM3 TN3
+    apply (drule spec[of _ u])
+    apply (drule spec[of _ u])
     apply safe
     subgoal for XM XN
       apply (rule exI[of _ "XM \<union> XN"])
-       apply (fastforce simp: cinfmset_map_comp intro!: arg_cong2[of _ _ _ _ image_cinfmset])
+      apply safe
+      using var_lam_pre_class.Un_bound apply blast
+      apply (auto intro!: arg_cong2[of _ _ _ _ iApp] arg_cong2[of _ _ _ _ image_cinfmset])
       done
     done
-  subgoal for lp1 lp2 M N TM2 TN2 TM1 TN1 u g a
-    apply (drule spec[of _ u])+
-    apply (drule mp, rule refl)+
-    apply fastforce
-    done
-  subgoal for lp1 lp2 x M TM1 TM2 u
-    apply (drule spec[of _ u])+
-    apply (drule mp, rule refl)+
+  subgoal for lp1 lp2 x M TM2 TM1 u TM3
+    apply (rotate_tac 2)
+    apply (drule spec[of _ u])
     apply safe
     subgoal for X
       apply (rule exI[of _ "X - {x}"])
-      apply (clarsimp simp add: ilam.map_id)
       apply safe
-      sorry
-    done
-  subgoal for lp1 lp2 x M TM1 TM2 u g a
-    apply (drule spec[of _ u])+
-    apply (drule mp, rule refl)+
-    apply auto
-    done
-  done
+      using card_of_minus_bound apply blast
+      apply (rule exists_fresh[THEN exE])
+       apply assumption
+      subgoal for g g' a z
+        find_theorems "iAbs _ _ = iAbs _ _"
+      find_theorems "_ <o _ \<Longrightarrow> \<exists> _. _ \<notin> _"
 
-lemma apply_super_comp_super[simp]: "bij f \<Longrightarrow> apply_super (comp_super g f) x = apply_super g (f x)"
+  thm ilam.card_of_FFVars_bounds
+  thm sum2.sum.rel_lam_presum
+ML \<open>Defs.specifications_of (Theory.defs_of @{theory}) (Defs.Const, @{const_name "sum2.sum.rel_lam_presum"})\<close>
+  find_theorems sum2.sum.rel_lam_presum
+
+
+lemma apply_super_comp_super[simp]: "apply_super (comp_super g f) x = apply_super g (f x)"
   apply transfer
   apply auto
   done
 
-lemma comp_super_swap_super[simp]: "bij f \<Longrightarrow>
-  comp_super (swap_super g z z') f =
-  swap_super (comp_super g f) (inv f z) (inv f z')"
-  by transfer fastforce
-
-lift_definition map_U_lam_ilam :: "('a \<Rightarrow> 'a) \<Rightarrow> 'a lam \<Rightarrow> 'a U_lam_ilam \<Rightarrow> 'a :: var_ilam_pre U_lam_ilam" is
-  "\<lambda>f t T g a. if bij f then T (comp_super g f) a else T g a"
-  apply safe
-  subgoal for f _ T X
-    apply (rule exI[of _ "if bij f then f ` X else X"])
-    apply (clarsimp simp add: fun_eq_iff)
-    subgoal for z z' g a
-    apply (drule spec[of _ "inv f z"])
-      apply (drule spec[of _ "inv f z'"])
-      apply (drule mp)
-       apply force
-      apply (drule spec2[of _ "comp_super g f" a])
-      apply auto
-      done
-    done
-  done
-
-lift_definition set_U_lam_ilam :: " 'a lam \<Rightarrow> 'a :: var_ilam_pre U_lam_ilam \<Rightarrow> 'a set" is
-  "\<lambda>t T. {x. \<exists>g g' a. T g a \<noteq> T g' a \<and> (\<forall>y. y \<noteq> x \<longrightarrow> apply_super g y = apply_super g' y)}"
-  .
-
 lemma map_CCTOR_lam_ilam:
   "bij f \<Longrightarrow>
-       |supp f| <o |UNIV| \<Longrightarrow>
-       map_U_lam_ilam f (lam_ctor (map_lam_pre id id fst fst y))
-        (CCTOR_lam_ilam y p) =
+       |supp (f :: 'a \<Rightarrow> 'a)| <o |UNIV :: 'a :: var_ilam_pre set| \<Longrightarrow>
+       (\<lambda>g. CCTOR_lam_ilam y p (comp_super g f)) =
        CCTOR_lam_ilam
         (map_lam_pre f f
-          (\<lambda>(t, pu). (rrename_lam f t, \<lambda>p. map_U_lam_ilam f t (pu (id p))))
-          (\<lambda>(t, pu). (rrename_lam f t, \<lambda>p. map_U_lam_ilam f t (pu (id p)))) y)
-        (id p)"
-  sorry
+          (\<lambda>(t, pu). (rrename_lam f t, \<lambda>p g. pu (id p) (comp_super g f)))
+          (\<lambda>(t, pu). (rrename_lam f t, \<lambda>p g. pu (id p) (comp_super g f))) y)
+        (id p) "
+  apply (auto simp: CCTOR_lam_ilam_def map_lam_pre_def Abs_lam_pre_inverse
+    cinfmset.map_comp o_def split: sum.splits prod.splits)
+  done
+
+definition "AbsT z T = (\<lambda>g a. iAbs (apply_super g z) (T g a))"
+
+definition "fvT T = {x. \<exists>g g'.
+           (\<exists>a. T g a \<noteq> T g' a) \<and>
+           (\<forall>y. y \<noteq> x \<longrightarrow> apply_super g y = apply_super g' y)}"
+
+lemma "fvT (AbsT z T) \<subseteq> fvT T - {z}"
+  unfolding AbsT_def fvT_def
+  apply auto
+  subgoal sorry
+  subgoal for g g' a
+    apply (erule notE)
+    apply (cases "g = g'")
+    apply auto
 
 lemma set_CCTOR_lam_ilam: "set2_lam_pre y \<inter> ({} \<union> {}) = {} \<Longrightarrow>
-  set2_lam_pre y \<inter> ({} \<union> {}) = {} \<Longrightarrow>
-       (\<And>t pu p. (t, pu) \<in> set3_lam_pre y \<union> set4_lam_pre y \<Longrightarrow> set_U_lam_ilam t (pu p) \<subseteq> fv t \<union> {} \<union> {}) \<Longrightarrow>
-       set_U_lam_ilam t (CCTOR_lam_ilam y p) \<subseteq> fv (lam_ctor (map_lam_pre id id fst fst y)) \<union> {} \<union> {}"
-  apply clarsimp
-  apply (auto simp: CCTOR_lam_ilam_def set_U_lam_ilam_def
+       (\<And>t pu p.
+           (t, pu) \<in> set3_lam_pre y \<union> set4_lam_pre y \<Longrightarrow>
+           {x. \<exists>g g' a. pu p g a \<noteq> pu p g' a \<and> (\<forall>y. y \<noteq> x \<longrightarrow> apply_super g y = apply_super g' y)}
+           \<subseteq> fv t \<union> {} \<union> {}) \<Longrightarrow>
+       {x. \<exists>g g' a.
+              CCTOR_lam_ilam y p g a \<noteq> CCTOR_lam_ilam y p g' a \<and> (\<forall>y. y \<noteq> x \<longrightarrow> apply_super g y = apply_super g' y)}
+       \<subseteq> fv (lam_ctor (map_lam_pre id id fst fst y)) \<union> {} \<union> {}"
+  apply (auto simp: CCTOR_lam_ilam_def
     Var_def[symmetric] Abs_def[symmetric] App_def[symmetric]
     map_lam_pre_def set3_lam_pre_def set4_lam_pre_def
-    Abs_lam_pre_inverse
+
  split: sum.splits prod.splits)
+     apply metis
+  subgoal
+  apply (erule contrapos_np) sorry
+   apply (erule contrapos_np)
+  subgoal for y t rec x g g' a
+    apply (drule meta_spec[of _ t])
+    apply (drule meta_spec[of _ p])
+    apply simp
+    apply (cases "x \<noteq> y")
+     apply simp
+     apply (smt (verit) mem_Collect_eq subsetD)
+    apply simp
+    apply (cases "rec p g a = rec p g' a")
+    apply (drule subsetD[of _ _ y])
+     apply auto
+    apply (rule exI[of _ g])
+    apply (rule exI[of _ g'])
+    apply auto
+    sorry
+   apply (erule contrapos_np)
+  subgoal for y t rec g g' a
+    apply (drule meta_spec[of _ t])
+    apply (drule meta_spec[of _ p])
+    apply simp
 
 
 local_setup \<open>fn lthy =>
@@ -599,8 +564,8 @@ let
   val model = {
     U = @{typ "'a :: var_ilam_pre U_lam_ilam"},
     fp_result = fp_res,
-    UFVars = [@{term "set_U_lam_ilam :: 'a lam \<Rightarrow> 'a U_lam_ilam \<Rightarrow> 'a :: var_ilam_pre set"}],
-    Umap = @{term "map_U_lam_ilam :: ('a \<Rightarrow> 'a) \<Rightarrow> 'a lam \<Rightarrow> 'a U_lam_ilam \<Rightarrow> 'a :: var_ilam_pre U_lam_ilam"},
+    UFVars = [@{term "(\<lambda>t T. {x. \<exists>g g' a. T g a \<noteq> T g' a \<and> (\<forall>y. y \<noteq> x \<longrightarrow> apply_super g y = apply_super g' y)}) :: 'a lam \<Rightarrow> 'a U_lam_ilam \<Rightarrow> 'a :: var_ilam_pre set"}],
+    Umap = @{term "(\<lambda>f t T g a. T (comp_super g f) a) :: ('a \<Rightarrow> 'a) \<Rightarrow> 'a lam \<Rightarrow> 'a U_lam_ilam \<Rightarrow> 'a :: var_ilam_pre U_lam_ilam"},
     Uctor = @{term CCTOR_lam_ilam},
     avoiding_sets = [ @{term "{} :: 'a::var_ilam_pre set"}],
     parameters = params,
